concur/InvariantC.v
@@ -1,0 +1,271 @@
+Require Import Values.
+Require Import AST.
+Require Import Globalenvs.
+Require Import Events.
+Require Import LanguageInterface.
+Require Import CallconvAlgebra.
+Require Import CKLR.
+Require Import Smallstep.
+
+Require Import Invariant.
+Require Import CallconvBig VCompBig.
+               
+(** ** Preservation *)
+
+(** A small step semantics preserves an externally observable
+  invariant if the following properties hold. In addition to the
+  invariant interfaces for the incoming function call ([IB]) and any
+  outgoing external calls ([IA]), we specify a "state invariant" [IS]
+  which will be estblished by the initial query and external call
+  returns, preserved by internal steps, and ensure the invariant
+  interface is respected at external calls and final states. *)
+
+Record lts_preserves {li S} se (L: lts li li S) I (IS: _ -> S -> Prop) w :=
+  {
+    preserves_step s t s':
+      IS w s ->
+      Step L s t s' ->
+      IS w s';
+    preserves_initial_state q s:
+      query_inv I w q ->
+      initial_state L q s ->
+      IS w s;
+    preserves_external s q:
+      IS w s -> at_external L s q ->
+      exists wA, symtbl_inv I wA se /\ query_inv I wA q /\
+      forall r s', reply_inv I wA r -> after_external L s r s' -> IS w s';
+    preserves_final_state s r:
+      IS w s ->
+      final_state L s r ->
+      reply_inv I w r;
+  }.
+
+Definition preserves {li} (L: semantics li li) (I: invariant _) IS :=
+  forall w se,
+    Genv.valid_for (skel L) se ->
+    symtbl_inv I w se ->
+    lts_preserves se (L se) I IS w.
+
+(** ** As calling conventions *)
+
+(** Invariant interfaces are essentially a unary version of calling
+  conventions, and can in fact be lifted into actual, binary calling
+  conventions asserting that the source and target queries are
+  identical, and furthermore satisfy the given invariant. *)
+
+Program Coercion cc_inv {li : language_interface} (I : invariant li) : GS.callconv li li :=
+  {|
+    GS.ccworld := inv_world I;
+    GS.ccworld_world := world_unit;
+    GS.match_senv := fun w => rel_inv (symtbl_inv I w);
+    GS.match_query := fun w => rel_inv (query_inv I w);
+    GS.match_reply := fun w => rel_inv (reply_inv I w)
+  |}.
+Next Obligation.
+  inv H. reflexivity.
+Qed.
+Next Obligation.
+  inv H. auto.
+Qed.
+
+
+(** With this, an invariant preservation proof can itself be lifted
+  into a self-simulation by the invariant calling conventions. *)
+
+Lemma preserves_fsim {li} (L: semantics li li) I IS:
+  preserves L I IS ->
+  GS.forward_simulation (cc_inv I) L L.
+Proof.
+  intros MATCH. constructor.
+  eapply GS.Forward_simulation; eauto.
+  intros se1 se2 w Hse Hse1. (eapply GS.forward_simulation_step with (match_states := fun _ => rel_inv (IS w));
+                                
+                                destruct Hse; subst).
+  - destruct 1. auto.
+  - intros q _ s [Hq] Hs.
+    exists s. split; eauto.
+    constructor.
+    eapply preserves_initial_state; eauto.
+  - intros gw s _ r [Hs] Hr.
+    exists r, tt. split; eauto.
+    constructor. reflexivity. split. reflexivity. constructor.
+    eapply preserves_final_state; eauto.
+  - intros gw s _ q [Hs] Hq.
+    edestruct @preserves_external as (wA & Hse & HqA & Hr); eauto.
+    exists wA, q. repeat apply conj; cbn; eauto.
+    + constructor. auto.
+    + constructor. auto.
+    + intros r' r'' s' t [Hr'] Hs'. inv H0.
+      exists s'. split; eauto.
+      econstructor.
+      eapply Hr; eauto.
+  - intros s t s' Hstep a b [Hs].
+    exists s'. split; eauto.
+    constructor.
+    eapply preserves_step; eauto.
+  - auto using well_founded_ltof.
+Qed.
+
+
+(** * Invariant-based simulation proof methods *)
+
+(** Once we have established that the source or target language
+  preserves an invariant of interest, we wish to use that fact to
+  help prove the forward simulation for the pass being considered.
+
+  The most basic way to do that is to add an assertion to the
+  simulation relation that the states satisfy the invariant. Then,
+  we rely on these assertions to prove a simulation step, and use the
+  relevant preservation lemmas to establish them again for the
+  successor states. This approach is workable and has been used in
+  CompCert for typing invariants, but it is somewhat ad-hoc and
+  becomes more involved when the interaction with the environment is
+  involved in the invariant's preservation.
+
+  Instead, we would like to formulate a weaker simulation diagram,
+  where the invariant can be assumed on the current states but does
+  not need to be established for the successor states, then show that
+  if the language involved [preserves] the invariant (in the sense
+  defined above), then this weakened diagram is sufficient to
+  establish a forward simulation for the pass.
+
+  The most straightforward way to do this would be to define a
+  weakened version of [forward_simulation] along these lines, however
+  this comes with its own pitfall: there already exists many lemmas
+  one can use to establish a [forward_simulation] using simplified
+  diagrams rather than the more complex, general form, and we would
+  like to be able to use simplified diagrams for our weakened version
+  as well. Under this approach, we would have to duplicate such lemmas
+  for the weakened diagram. Instead, the method implemented below
+  reuses [forward_simulation] and expresses the weakened diagram as a
+  special case, making it possible to reuse all existing techniques to
+  prove it.
+
+  Since by definition, [forward_simulation] uses the same simulation
+  relation for the current and successor states, we accomplish this by
+  acting on the transition systems themselves:
+
+    - for the source language, we can build a strengthened version of
+      the transition system which restricts the transitions to states
+      which statisfy the invariant;
+    - for the target language, we can build a relaxed version of the
+      transition system which adds arbitrary transitions from states
+      which do not satisfy the invariant.
+
+  Proving a simulation from the strengthened source semantics, and/or
+  to the weakened target semantics, is easier because we have
+  hypotheses that the states involved satify the invariant. At the
+  same time, for an invariant-preserving language, we can easily show
+  a simulation from the original to the strengthened version, and from
+  the weakened to the original version, and these simulations can be
+  composed with that proved by the user to obtain the desired one. *)
+
+(** ** Strengthening the source semantics *)
+
+
+Section RESTRICT.
+  Context {li} (L: semantics li li).
+  Context (I: invariant li).
+  Context (IS: inv_world I -> state L -> Prop).
+
+  Definition restrict_lts se :=
+    {|
+      step ge s t s' :=
+        step (L se) ge s t s' /\
+        exists w,
+          symtbl_inv I w se /\
+          IS w s /\
+          IS w s';
+      valid_query q :=
+        valid_query (L se) q;
+      initial_state q s :=
+        initial_state (L se) q s /\
+        exists w,
+          symtbl_inv I w se /\
+          query_inv I w q /\
+          IS w s;
+      final_state s r :=
+        final_state (L se) s r /\
+        exists w,
+          symtbl_inv I w se /\
+          IS w s /\
+          reply_inv I w r;
+      at_external s q :=
+        at_external (L se) s q /\
+        exists w wA,
+          symtbl_inv I w se /\
+          IS w s /\
+          query_inv I wA q;
+      after_external s r s' :=
+        after_external (L se) s r s' /\
+        exists w wA q,
+          symtbl_inv I w se /\
+          at_external (L se) s q /\
+          IS w s /\
+          query_inv I wA q /\
+          reply_inv I wA r /\
+          IS w s';
+    globalenv :=
+      globalenv (L se);
+  |}.
+
+  Definition restrict :=
+    {|
+      skel := skel L;
+      state := state L;
+      (* memory_of_state := memory_of_state L; *)
+      activate se := restrict_lts se;
+    |}.
+
+  Lemma restrict_fsim:
+    preserves L I IS ->
+    GS.forward_simulation (cc_inv I) L restrict.
+  Proof.
+    intro MATCH. econstructor.
+    econstructor. reflexivity.
+    intros se1 sae2 w Hse Hse1. eapply GS.forward_simulation_step with (match_states := fun _ =>rel_inv (IS w));(destruct Hse; subst); cbn; auto.
+    - destruct 1. reflexivity.
+    - intros q _ s [Hq] Hs. exists s.
+      assert (IS w s) by (eapply preserves_initial_state; eauto).
+      eauto 10 using rel_inv_intro.
+    - intros gw s _ r [Hs] Hr. exists r.
+      assert (reply_inv I w r) by (eapply preserves_final_state; eauto).
+      eauto 10 using rel_inv_intro.
+    - intros tt s _ q [Hs] Hx.
+      edestruct @preserves_external as (wA & HseA & Hq & Hk); eauto.
+      eexists wA, q. intuition eauto 10 using rel_inv_intro.
+      destruct H3. exists s1'. intuition eauto 20 using rel_inv_intro.
+    - intros s t s' STEP a b [Hs].
+      assert (IS w s') by (eapply preserves_step; eauto).
+      exists s'. eauto 10 using rel_inv_intro.
+    - auto using well_founded_ltof.
+  Qed.
+
+  Lemma restrict_determinate:
+    determinate L ->
+    determinate restrict.
+  Proof.
+    intros HL se. specialize (HL se) as [ ].
+    split; unfold nostep, not, single_events in *; cbn; intros;
+    repeat (lazymatch goal with H : _ /\ _ |- _ => destruct H as [H _] end);
+    eauto.
+  Qed.
+End RESTRICT.
+  
+Infix "@" := GS.cc_compose (at level 30, right associativity).
+
+Section METHODS.
+  Context {li1 li2} {cc: GS.callconv li1 li2}.
+  Context (L1: semantics li1 li1) (L2: semantics li2 li2).
+
+  Lemma source_invariant_fsim I IS:
+    preserves L1 I IS ->
+    GS.forward_simulation cc (restrict L1 I IS) L2 ->
+    GS.forward_simulation (I @ cc) L1 L2.
+  Proof.
+    intros HL1 HL.
+    eapply st_fsim_vcomp; eauto.
+    apply restrict_fsim; auto.
+  Qed.
+
+End METHODS.
